Add spec and proof for iterator_find
Signed-off-by: Ike Mulder <ikemul@amazon.com>

Micro_Rust_Std_Lib/StdLib_Iterators.thy
@@ -72,6 +72,41 @@ instance ..
 
 end
 
+
+definition iterator_find_contract :: \<open>'a list \<Rightarrow> ('a \<Rightarrow> bool) \<Rightarrow>
+  ('machine::sepalg, 'abort, 'i, 'o) striple_context \<Rightarrow>
+  ('a \<Rightarrow> ('machine, bool, 'abort, 'i prompt, 'o prompt_output) function_body) \<Rightarrow>
+  ('machine, 'a option, 'abort) function_contract\<close> where
+  \<open>iterator_find_contract vs pred_pure \<Gamma> pred_rust \<equiv>
+    let pre = \<langle>\<forall> i. \<Gamma>; pred_rust i \<Turnstile>\<^sub>F lift_pure_to_contract (pred_pure i)\<rangle> in
+    let post = \<lambda> ret. \<langle>ret = List.find pred_pure vs\<rangle> in
+    make_function_contract pre post\<close>
+ucincl_auto iterator_find_contract
+
+declare lift_pure_to_contract_def [crush_contracts]
+ucincl_auto lift_pure_to_contract
+
+lemma iterator_find_spec:
+  shows \<open>\<Gamma> ; StdLib_Iterators.find (make_iterator_from_list vs) pred_rust \<Turnstile>\<^sub>F iterator_find_contract vs pred_pure \<Gamma> pred_rust\<close>
+proof (crush_boot f: StdLib_Iterators.find_def contract: iterator_find_contract_def, goal_cases)
+  case 1
+  note pred_spec = this[THEN spec]
+  show ?case proof (crush_base inline: iterator_into_iter_def, induction vs)
+    case Nil
+    then show ?case
+      by (crush_base simp add: raw_for_loop_def)
+  next
+    case (Cons a vs)
+    note IH = this
+    show ?case
+      apply (crush_base specs add: pred_spec)
+      apply (cases \<open>pred_pure a\<close>)
+       apply crush_base
+      apply (subst List.find.simps(2), simp)
+      by (rule IH)
+  qed
+qed
+
 (*<*)
 end
 (*>*)
